

Surreal # ($\mathcal{S} := \{\text{all the surreal \#s}\}$)

Part 1 Definitions.

Def 1: A Surreal number x is a pair of previously created surreal numbers, known as the left set X_L and the ~~left~~^{right} set X_R with no member of the right set may be less than or equal to any member of X_L .

Def 2: $x, y \in \mathcal{S}$ $x \leq y$ iff the followings:

$$\bullet \neg \exists x_L \in X_L : y \leq x_L \quad (*1)$$

$$\bullet \neg \exists y_R \in Y_R : y_R \leq x \quad (*2)$$

Def (zero). We define zero as: $0 := \{\} := \{\emptyset | \emptyset\}$

Thm 1: $0 \leq 0$

Proof: Since O_L and O_R are empty, then the conditions in def 2 holds. $\Rightarrow 0 \leq 0$ \square

Def $-1 := \{0\}$, $1 := \{0\}$.

Rmk: Check the well-definedness of -1 and 1 . Since $(-1)_L$ and $(1)_R$ are empty, then the condition for well-definedness in def 1 holds naturally.

Thm $0 \leq 1$ and $-1 \leq 0$

Proof: For " $0 \leq 1$ ", O_L & 1_R are empty. Then " $0 \leq 1$ " holds. For " $-1 \leq 0$ ", $(-1)_L$ and O_R are empty. Then " $-1 \leq 0$ " holds. Hence, we're done. \checkmark

Notational Conventions

$x \neq y$ means $\neg(x \leq y)$

$x < y$ means $x \leq y$ and $y \neq x$

$x \not\leq y$ means $\neg(x \leq y) \Leftrightarrow x \neq y \vee y \leq x$

$x = y$ means $x \leq y$ and $y \leq x$

$x \neq y$ means ~~$\neg(x = y)$~~ $\neg(x = y)$

Theorem, $0 = 0$

Proof: $0 \leq 0$ and $0 \leq 0 \Rightarrow 0 = 0$

Thm: $\textcircled{1} 1=1, \textcircled{2} -1=-1, \textcircled{3} 0<1, \textcircled{4} -1<0, \textcircled{5} -1<1$

Proof:

① W.T.S: $1 \leq 1 \iff \underbrace{\neg \exists x \in 1_L : 1 \leq x}_{(i)} \wedge \underbrace{\neg \exists y \in 1_R : y \leq 1}_{(ii)}$

Since $\cancel{1_R} = \emptyset$, then (ii) holds. For (i), $1_L = \{0\}$, so (i) holds because $0 \leq 1$ by the previous thm.

$$\textcircled{2} \quad \underbrace{\neg \exists x \in (-1)_L : \neg \leq x} \wedge \underbrace{\neg \exists y \in (-1)_R : y \leq -1}_{\neg \{iv\}}$$

Since $(-1)_L = \emptyset$, then (iii) holds. For (iv), $(-1)_R = \{0\}$, so (iv) holds because $-1 \leq 0$ by the previous thm.

② W.T.S: $1 \neq 0 \Leftrightarrow \neg(1 \leq 0) \Leftrightarrow \exists x \in 1_L: 0 \leq x \vee \exists y \in 0_R: y \leq 1$

Since $I_L = \{0\}$ and $0 \leq 0$, then " $\exists x \in I_L: 0 \leq x$ " holds.

④ W.T.S.: $0 \not\leq -1 \Leftrightarrow \exists \alpha \in \mathcal{O}_L: -1 \leq \alpha \wedge \nexists \beta \in (-1)_K: \beta \leq 0$

Since $(-1)_R = \{0\}$ and $0 \leq 0$, then " $\exists y \in (-1)_R: y \leq 0$ " holds.

⑤ W.T. S: $-1 \leq 1 \wedge 1 \neq -1$

$$(a) \quad \neg \exists x \in (-1)_L = \emptyset \wedge \neg \exists y \in \mathbb{1}_R = \emptyset \Rightarrow \neg \exists x \in (-1)_L : x \leq 1 \wedge \neg \exists y \in \mathbb{1}_R : y \leq 1$$

$$\Rightarrow -1 \leq 1$$

(b) $1 \leq 0 \Rightarrow \exists x \in \mathbb{Z} = \{\delta\} \ (x=0): -1 \leq 0x \Rightarrow 1 \neq -1$ □

Def $z \equiv \{11\}$, $-z \equiv \{1-1\}$, $\frac{1}{z} \equiv \{011\}$, $-\frac{1}{z} \equiv \{-10\}$

Remark: The well-definedness of $2, -2, \frac{1}{2}, -\frac{1}{2}$ can be easily check by the thms on the left side of this page.

Then $O = \{-1, 1\}$

Proof:

① $0 \leq \{-1|1\}$: $\neg \exists x \in O_L = \emptyset$ ~~$\neg \exists x \in$~~ $\Rightarrow \exists x \in O_L: \{-1|1\} \leq x$

$$0 < 1 \Rightarrow 1 \neq 0 \Rightarrow \neg \exists y \in \mathbb{R} : y \leq 0$$
$$\Rightarrow \neg \exists y \in \{-11\}_{\mathbb{R}} : y \leq 0 \quad \text{---} (\#2)$$

Then by (#1) (#2), $0 \leq \{-1\}^2$

② $\{ -1 | 1 \} \leq 0 :$

$$\neg \exists x \in O_R = \emptyset \Rightarrow \neg \exists y \in O_R: y \leq \{-1, 1\}$$
$$\neg 1 < 0 \Rightarrow 0 \nless 1 \Rightarrow \neg \exists x \in \{-1\}: 0 \leq x$$
$$\Rightarrow \neg \exists x \in \{-1, 1\}_L : 0 \leq x \quad (*)_2$$

By $(*)1)(*)2)$, $\{-1|1\} \leq 0$

Then by ①②, we get that $0 = \{-1, 1\}$. \square

Def (Representative).

The different forms that represent the same surreal number are called representatives of that surreal number.

Example: $\{|\}$ and $\{-1|1\}$ are two representatives of the surreal number 0.

Def (Birthday)

- $0 \equiv \{|\}$ is born on day 0
- $-1 \equiv \{|\emptyset\}$, $1 \equiv \{\emptyset|\}$ are born on day 1.
- \vdots

Part 2 Basic Properties of Surreal Numbers

Def (Set comparisons). Let A be a set of surreal numbers, c be a surreal number. Then we define:

$$A \leq c \Leftrightarrow \forall a \in A: a \leq c$$

$$c \leq A \Leftrightarrow \forall a \in A: c \leq a$$

$$A \leq B \Leftrightarrow \forall a \in A, \forall b \in B: a \leq b.$$

Similarly for $A < c$, $A \neq B$.

Rank: $\neg(A \leq b)$ is NOT equivalent to $A \neq b$

Example: " $\{3, 5\} \leq 4$ " is false $\Rightarrow \neg(\{3, 5\} \leq 4)$ is true

However, $\{3, 5\} \neq 4$ is also false.

$\Rightarrow (\{3, 5\} \neq 4)$ is NOT equivalent to $\neg(\{3, 5\} \leq 4)$.

Def (Set Equality) $A, B \subseteq \mathcal{S}$.

$$A = B \Leftrightarrow (\forall a \in A \exists b \in B: a = b) \wedge (\forall b \in B \exists a \in A: b = a).$$

Rank: A and B are not necessarily identical forms.

Example: $\{\{1\}, \{1|\}\} = \{\{-1|1\}, \{1\}, \{-1, 0, 1|\}\}$,

since $\{1\} = \{-1|1\}$, $\{1\} = \{1\}$, $\{1|\} = \{-1, 0, 1|\}$.

Thm (Alternative Form of Comparison)

Let $x = \{X_L | X_R\}$, $y = \{Y_L | Y_R\}$ Then

$$x \leq y \Leftrightarrow (Y_R \neq x) \wedge (y \leq X_L)$$

where $\begin{cases} Y_R \neq x \text{ means } \neg \exists y_R \in Y_R: y_R \leq x \\ y \leq X_L \text{ means } \neg \exists x_L \in X_L: y \leq x_L. \end{cases}$

Rank: It's just a notational rewriting of Def 2.

Def (Parents (or Options))

The members of the left set \bar{X}_L and the right set \bar{X}_R of a surreal number $x = \{\bar{X}_L | \bar{X}_R\}$ are called the parents (or options) of x .

Thm (Reflexivity of \leq) If $x \in S$, then $x \leq x$.

Proof: By induction.

Basic Case: $0 \leq 0$, which we've shown

Inductive Step: Suppose that for all parents of x , the thm holds, that is, $\forall x_L \in \bar{X}_L$ & $\forall x_R \in \bar{X}_R$ we have $x_L \leq x_L$ & $x_R \leq x_R$. W.T.S.: $x \leq x$

$$\Leftrightarrow \underbrace{\neg \exists x_L \in \bar{X}_L : x \leq x_L}_{(i)} \wedge \underbrace{\neg \exists x_R \in \bar{X}_R : x_R \leq x}_{(ii)}$$

For (i), suppose not, i.e.: $\exists x_L \in \bar{X}_L : x \leq x_L$

$$\Rightarrow \neg \exists x'_L \in \bar{X}_L : x_L \leq x'_L \wedge \neg \exists x_{LR} \in \bar{X}_{LR} : x_{LR} \leq x$$

Since $x_L \leq x_L$, then let $x'_L = x_L$. Then contradict!

Hence, (i) is true. Similarly, (ii) is true. \square

Coro (Reflexivity of $=$). If $x \in S$, then $x = x$.

Proof: $x \leq x$ & $x \geq x \Rightarrow x = x$, by def of " $=$ ". \square

Thm Let A, A', B, B' be sets of surreal numbers, and let a_1, a_2, \dots be the members of A , let a'_1, a'_2, \dots be the members of A' , let b_1, b_2, \dots be the members of B , let b'_1, b'_2, \dots be the members of B' . If $\forall a_i \in A, \exists a'_j \in A'$ s.t.: $a_i \leq a'_j$ and $\forall b_k \in B \exists b'_p \in B'$ s.t.: $b_k \leq b'_p$, then $\{A|B\} \leq \{A'|B'\}$

Proof: W.T.S.: $\underbrace{\neg \exists a \in A : \{A'|B'\} \leq a}_{(i)} \wedge \underbrace{\neg \exists b' \in B' : b' \leq \{A|B\}}_{(ii)}$

For (i), suppose that $\exists a \in A : \{A'|B'\} \leq a$. Then

$\neg \exists a' \in A' : a \leq a'$. Contradict! \Rightarrow (i) holds.

For (ii), suppose that $\exists b' \in B' : b' \leq \{A|B\}$. Then

$\neg \exists b \in B : b' \leq b$, Contradict! \Rightarrow (ii) holds. \square

Coro. If $A = A'$ and $B = B'$, then $\{A|B\} = \{A'|B'\}$

Proof: $A = A' \Rightarrow \forall a \in A, \exists a' \in A'$ s.t.: $a = a' \Rightarrow a \leq a'$. Similarly for B and $B' \Rightarrow \{A|B\} \leq \{A'|B'\}$ & $\{A'|B'\} \leq \{A|B\}$ \square

Thm Let $x = \{A|B\}$ be a surreal number. Then

$\forall a \in A: a < x$ and $\forall b \in B: x < b$, that is,

$A < x$ and $x < B$.

Proof: W.T.S.: ~~A~~ $\left\{ \begin{array}{l} (a) \forall a \in A: a < x \Leftrightarrow \overset{(a1)}{a \leq x} \wedge \overset{(a2)}{a \neq x} \\ (b) \forall b \in B: x < b \Leftrightarrow \overset{(b1)}{x \leq b} \wedge \overset{(b2)}{b \neq x} \end{array} \right.$

(a1): $a \leq x \Leftrightarrow \underbrace{\neg \exists q_L \in A_L: x \leq q_L}_{\text{holds by def 1}} \wedge \underbrace{\neg \exists b \in B: b \leq a}_{\text{holds by def 1}}$

Suppose $\exists q_L \in A_L: x \leq q_L$. Then $\neg \exists a \in A: q_L \leq a$, which contradicts to the inductive step. \Rightarrow (a1) holds.

(a2): W.T.S.: $x \neq a \Leftrightarrow \neg(x \leq a) \Leftrightarrow \exists a' \in A: a \leq a' \wedge \forall b \in B: a \leq b$

The right-hand-side holds by def 1. \Rightarrow (a2) holds

(b1): $x \leq b \Leftrightarrow \underbrace{\neg \exists a \in A: a \leq b}_{\text{holds by def 1}} \wedge \neg \exists b_R \in B_R: b_R \leq x$

Suppose $\exists b_R \in B_R: b_R \leq x$. Then $\neg \exists b \in B: b \leq b_R$, which contradicts to the inductive step. \Rightarrow (b1) holds.

(b2): W.T.S.: $b \neq x \Leftrightarrow \neg(b \leq x) \Leftrightarrow \exists b_L^* \in B_L^*: b \leq b_L^* \wedge \forall b' \in B: b \leq b'$

By inductive step, left-hand-side holds \Rightarrow (b2) holds.

Then we're done.

Coro. If $x = \{a|\}$, then $a < x$.

Thm (Transitive law for \leq). If $x, y, z \in \mathcal{S}$, then $x \leq y \wedge y \leq z$ can imply $x \leq z$.

Proof: Suppose not, i.e.: $x \neq z$ when $x \leq y$ & $y \leq z$.

Take $p(x, y, z) \Leftrightarrow x \leq y \wedge y \leq z \wedge x \neq z$. Then

$\neg \exists x_L \in X_L: y \leq x_L$ (1); $\neg \exists y_R \in Y_R: y_R \leq x$ (2);

$\neg \exists y_L \in Y_L: z \leq y_L$ (3); $\neg \exists z_R \in Z_R: z_R \leq y$ (4);

$\exists x_L \in X_L: z \leq x_L \vee \exists z_R \in Z_R: z_R \leq x$.

Case 1: $\exists x_L \in X_L: z \leq x_L$. By (1), we have

$p(y, z, x_L) \Leftrightarrow y \leq z \wedge y \leq x_L \wedge y \neq x_L$

Case 2: $\exists z_R \in Z_R: z_R \leq x$. By (4), we have

$p(z_R, x, y) \Leftrightarrow z_R \leq x \wedge x \leq y \wedge z_R \neq y$

Hence, we have $p(x, y, z) \Leftrightarrow \exists x_L \in X_L: p(y, z, x_L) \vee$

$\exists z_R \in Z_R: p(z_R, x, y)$

Note that x_L, z_R are the parents of x and z respectively. Then by induction, we can prove it.

~~Basic case: $0 \leq 0$ & $0 \leq 0 \Rightarrow 0 = 0$.~~

~~Inductive step: Suppose that the transitive law~~

~~holds for all parents of x, y, z . Then~~

~~$p(x, y, z) \Leftrightarrow \exists x_L \in X_L: p(y, z, x_L) \vee \exists z_R \in Z_R: p(z_R, x, y)$~~

Then repeat that ~~proof~~ procedure and we
~~we~~ will reach 0. Then we have contradiction,
since $p(0,0,0)$ ~~is~~ ^{is} false. Hence, the assumption
never holds. Then we're done. \square